books/projects/rp-rewriter/proofs/extract-formula-lemmas.lisp
@@ -1677,7 +1677,7 @@
                     (rp-termp (RP-RHSm RULE))
                     (NOT (INCLUDE-FNC (RP-RHSm RULE) 'FALIST))
                     (NOT (INCLUDE-FNC (RP-HYPm RULE) 'FALIST))
-                    (NOT (INCLUDE-FNC (RP-LHSm RULE) 'IF))
+                    ;;(NOT (INCLUDE-FNC (RP-LHSm RULE) 'IF))
                     (NOT (INCLUDE-FNC (RP-LHSm RULE) 'SYNP))
                     (NO-FREE-VARIABLEP RULE)))
       :rule-classes :forward-chaining
